ironfleet/src/Dafny/Distributed/Protocol/RSL/FailureProof/FailureDetection_helper1.i.dfy
@@ -117,6 +117,44 @@ lemma NonSuspector0_ind(s:TimestampedRslState, s':TimestampedRslState, sr:set<in
 // NonSuspector2 inductive
 ////////////////////////////////////////////////////////////////////////////////
 
+lemma NonSuspector2_ind_7(s:TimestampedRslState, s':TimestampedRslState, sr:set<int>, j:int)
+  requires RslAssumption2(s, s')
+  requires EpochTimeoutQDInv(s)
+  requires EpochTimeoutQDInv(s')
+  requires 0 <= j < |s.constants.config.replica_ids|;
+
+  requires s.t_environment.nextStep.LEnvStepHostIos?;
+  requires s.t_environment.nextStep.actor == s.constants.config.replica_ids[j];
+
+  requires TimestampedRslNextOneReplica(s, s', j, s.t_environment.nextStep.ios);
+  requires s.t_environment.nextStep.nodeStep == RslStep(7);
+
+  requires InView1(s, sr);
+  requires j !in sr;
+  requires NonSuspector2(s, j);
+
+  ensures  NonSuspector2(s', j) || NonSuspector0(s', j) || InternalSuspector3(s', j);
+  ensures NotKnownSuspector(s', j);
+{
+  var ios := s.t_environment.nextStep.ios;
+  var clock := SpontaneousClock(UntagLIoOpSeq(ios));
+  var es := s.t_replicas[j].v.replica.proposer.election_state;
+  if clock.t < es.epoch_end_time {
+    assert NotKnownSuspector(s', j);
+    assert NonSuspector2(s', j);
+  } else {
+    if j == 1 {
+      assert NotKnownSuspector(s', j); // might not be true
+      assert InternalSuspector3(s', j);
+      // FIXME: might go straight to InFinalState(), if j == 1 is the leader
+    } else {
+      assert NotKnownSuspector(s', j); // might not be true
+      assert InternalSuspector3(s', j);
+      // FIXME: prove TimeLe() using Heartbeat lemmas
+    }
+  }
+}
+
 lemma NonSuspector2_ind(s:TimestampedRslState, s':TimestampedRslState, sr:set<int>, j:int)
   requires RslAssumption2(s, s')
   requires EpochTimeoutQDInv(s)
@@ -134,10 +172,12 @@ lemma NonSuspector2_ind(s:TimestampedRslState, s':TimestampedRslState, sr:set<in
 
   ensures  NonSuspector2(s', j) || NonSuspector0(s', j)
     || InternalSuspector3(s', j);
+
   ensures NotKnownSuspector(s', j);
 {
   var step := s.t_environment.nextStep.nodeStep;
   if step == RslStep(6) {
+    assert NotKnownSuspector(s', j);
     if s.t_replicas[j].v.replica.executor.next_op_to_execute.OutstandingOpKnown? {
       var es := s.t_replicas[j].v.replica.proposer.election_state;
       var es' := s'.t_replicas[j].v.replica.proposer.election_state;
@@ -152,18 +192,26 @@ lemma NonSuspector2_ind(s:TimestampedRslState, s':TimestampedRslState, sr:set<in
           es.requests_received_prev_epochs,
           batch);
 
-        // assert (req in es.requests_received_this_epoch) && RequestsMatch(req, newReq);
-        assert es'.requests_received_prev_epochs == [];
-        assert es'.requests_received_this_epoch == [];
-        assert NonSuspector0(s', j);
-        return;
+        if es'.requests_received_prev_epochs == [] {
+          assert es'.requests_received_this_epoch == [];
+          assert NonSuspector0(s', j);
+          return;
+        } else {
+          assert NonSuspector2(s', j);
+        }
       }
     }
     assert NonSuspector2(s', j);
   } else if step == RslStep(7) {
-    assert false;
+    NonSuspector2_ind_7(s, s', sr, j);
+  } else if step == RslStep(8) {
+    var r := s.t_replicas[j].v.replica;
+    SubsetCardinality(r.proposer.election_state.current_view_suspectors, sr);
+    assert NonSuspector2(s', j);
+    assert NotKnownSuspector(s', j);
   } else {
     assert NonSuspector2(s', j);
+    assert NotKnownSuspector(s', j);
   }
 }
 
